Makefile
@@ -2,7 +2,8 @@
 # System configuration
 
 # You can build anything reachable from these root files.
-DAFNY_ROOTS=concurrency/scache/Bundle.i.dfy
+DAFNY_ROOTS=concurrency/scache/Bundle.i.dfy \
+						concurrency/node-replication/Impl.i.dfy
 
 DAFNY_ROOT?=.dafny/dafny/
 DAFNY_CMD=$(DAFNY_ROOT)/Scripts/dafny
